# extranious solutions 
### $2 \sqrt{x+4}-1 = x$
cancel the -1 out, getting $2 \sqrt{x+4} = x+1$                          
square both sides, getting  $4(x+4) = (x+1)(x+1)$ , or $4x+16 = x^2 + 2x +1$                  
get all onto one side by subtracting 4x+16 from both ends, getting $0 = x^2-2x-15$              
factor that into $(x-5)(x+3)$, then see what makes those 0, it would be +5 and -3, plug those into the OG problem and see if true, if true answer is valid and if wrong answer is extraneous        

# Inverses
$g(x)=3x^4$ or $y=3x^4$            
replace Y with X and vice versa getting $x=3y^4$        
now get Y alone divide by three getting $\frac{x}{3}=y^4$
4th root both sides getting $\sqrt{\frac{X}{3}}=Y$ (pretend its a fourth root) but you cant have a denomiator root....
multiply it to make a perfect 4th root, in this case 81, and 3*27 makes 81 so make this mess : $\sqrt{\frac{X}{3}} = \frac{\sqrt{x}}{\sqrt{3}} * \frac{\sqrt27}{\sqrt27} = \frac{\sqrt{{27x}}}{\sqrt81} = \frac{\sqrt27x}{3}$            
> [!NOTE]
> Pretend all the $\sqrt{.}$ are actually 4th roots and not squared roots

# EXoponets notes
Allways add
