# X^2<>Number

how to solve this 4x^2<25

Subtract 25 from both sides of the inequality:

4x^2 - 25 < 0

Factor the left side of the inequality:

Recognize that 4x^2 - 25 can be written as (2x)^2 - 5^2, which is in the form of the difference of squares.

Apply the difference of squares formula, which states that a^2 - b^2 = (a + b)(a - b). In this case, a is 2x, and b is 5.

Use the formula to factor 4x^2 - 25:

4x^2 - 25 = (2x + 5)(2x - 5)

So, the expression 4x^2 - 25 can be factored as (2x + 5)(2x - 5).

(2x + 5)(2x - 5) < 0

Now, you need to find the values of x that make the expression (2x + 5)(2x - 5) less than 0. To do this, you can use the sign of the factors. The sign changes at the roots of each factor, which are x = -5/2 and x = 5/2.

Create a sign chart with these critical values:

![wasd](https://github.com/Ethan-Ryan-Anderson/School-Notes-23-24-SMFHS/assets/118407438/3fde5571-256d-4163-913b-c418f9fd1ea3)


The inequality (2x + 5)(2x - 5) is less than 0 in the intervals where the sign chart shows a negative sign. So, the solution to the inequality is:

x < -5/2 or 5/2 < x

This means that x can be any real number less than -5/2 or greater than 5/2 for the inequality 4x^2 < 25 to be satisfied.

# X^2 - NumX <> Numb

To solve the quadratic inequality x^2 - 11x ≥ -28, you can follow these steps and explain how to factor it along the way:

Start with the quadratic inequality:

x^2 - 11x ≥ -28

Move all terms to one side of the inequality to set it equal to zero:

x^2 - 11x + 28 ≥ 0

To factor this quadratic expression, you need to find two numbers that multiply to the coefficient of x^2 (which is 1) times the constant term (which is 28), and these two numbers must add up to the coefficient of the linear term (which is -11). These numbers are -7 and -4 because (-7) * (-4) = 28, and (-7) + (-4) = -11.

Rewrite the middle term (-11x) using these two numbers as coefficients:

x^2 - 7x - 4x + 28 ≥ 0

Group and factor by grouping:

(x^2 - 7x) - (4x - 28) ≥ 0

Factor each group:

x(x - 7) - 4(x - 7) ≥ 0

Notice that (x - 7) is a common factor:

(x - 7)(x - 4) ≥ 0

You have successfully factored the quadratic expression as (x - 7)(x - 4) ≥ 0. Now, you can proceed to solve the inequality.

To find the solutions to the inequality, consider the critical points where the expression (x - 7)(x - 4) changes sign. These critical points are x = 4 and x = 7. Create a sign chart with these critical values and test intervals as explained in the previous response to determine the solutions to the inequality. The solution is:

x ≤ 4 or x ≥ 7

This means that x can be any real number less than or equal to 4 or greater than or equal to 7 for the inequality x^2 - 11x ≥ -28 to be satisfied.

# Frac(x)^2 numx <> num
Solving the quadratic inequality (1/2)x^2 - x > 4 involves the same general approach as before, but the coefficient of x^2 is different. Let's go through the steps:

Start with the quadratic inequality:

(1/2)x^2 - x > 4

To remove the fraction, you can multiply the entire inequality by 2 to get rid of the fraction:

x^2 - 2x > 8

Move all terms to one side of the inequality to set it equal to zero:

x^2 - 2x - 8 > 0

To factor this quadratic expression, you need to find two numbers that multiply to the coefficient of x^2 (which is 1) times the constant term (which is -8), and these two numbers must add up to the coefficient of the linear term (which is -2). These numbers are -4 and 2 because (-4) * (2) = -8, and (-4) + (2) = -2.

Rewrite the middle term (-2x) using these two numbers as coefficients:

x^2 - 4x + 2x - 8 > 0

Group and factor by grouping:

(x^2 - 4x) + (2x - 8) > 0

Factor each group:

x(x - 4) + 2(x - 4) > 0

Notice that (x - 4) is a common factor:

(x - 4)(x + 2) > 0

Now that you've factored the quadratic expression as (x - 4)(x + 2) > 0, you can proceed to solve the inequality.

To find the solutions to the inequality, consider the critical points where the expression (x - 4)(x + 2) changes sign. These critical points are x = -2 and x = 4. Create a sign chart with these critical values and test intervals to determine the solutions to the inequality. The solution is:

x < -2 or x > 4

This means that x can be any real number less than -2 or greater than 4 for the inequality (1/2)x^2 - x > 4 to be satisfied.

# (num ± num(i)) ± (num ± num(i))
To solve the expression (3 - 6i) - (7 + 2i), you are performing complex number subtraction. Follow these steps:

Subtract the real parts (the parts without the "i") and the imaginary parts separately:

Real part: 3 - 7 = -4
Imaginary part: -6i - 2i = -8i

Combine the results from step 1 to form the complex number:

-4 - 8i

So, (3 - 6i) - (7 + 2i) equals -4 - 8i.

# (num ± num(i) (num ± num(i)
To multiply the complex numbers (5 + 6i) and (-4 + 7i), you can use the distributive property. Here are the steps:

Multiply the real parts together (5 and -4):

Real part: (5) * (-4) = -20

Multiply the real part of the first complex number by the imaginary part of the second complex number (5 and 7i):

-20 + 35i

Multiply the imaginary part of the first complex number by the real part of the second complex number (6i and -4):

-24i

Multiply the imaginary parts together (6i and 7i):

Imaginary part: (6i) * (7i) = 42i^2

Combine the results from steps 2, 3, and 4:

-20 + 35i - 24i + 42i^2

Since i^2 is equal to -1, replace i^2 with -1:

-20 + 35i - 24i - 42

Combine like terms:

-62 + 11i

So, the product of (5 + 6i) and (-4 + 7i) is -62 + 11i.

# Num(x)^2 + num = 0

To solve the quadratic equation 7x^2 + 21 = 0, you can follow these steps:

Subtract 21 from both sides of the equation to isolate the quadratic term:

7x^2 = -21

Divide both sides by 7 to solve for x^2:

x^2 = -21 / 7

Simplify the right side:

x^2 = -3

Take the square root of both sides to solve for x:

x = ±√(-3)

However, the square root of a negative number is not a real number, so in this case, there are no real solutions. The solutions are complex and can be expressed as:

x = ±√3 * i

Where 'i' is the imaginary unit.

# Finding Zeros

here are the steps to find the zeros of f(x) = 2x^2 + 32:

Start with the equation: 2x^2 + 32 = 0.

Subtract 32 from both sides: 2x^2 = -32.

Divide both sides by 2: x^2 = -16.

Take the square root of both sides: x = ±√(-16).

Since the square root of -16 is not a real number, it involves the imaginary unit i: x = ±4i.

So, the zeros of the function are x = ±4i.

# Completing Square 


To solve the quadratic equation x^2 + 16x + 17 = 0 by completing the square, follow these steps:

Start with the equation: x^2 + 16x + 17 = 0.

Move the constant term to the other side of the equation (subtract 17 from both sides): x^2 + 16x = -17.

To complete the square, we want the coefficient of x^2 to be 1, so divide the entire equation by 1: (1)x^2 + 16x = -17.

Now, to complete the square, add and subtract (1/2)^2 to the x terms. This is done because (1/2)^2 = 1/4, and we're adding and subtracting to keep the equation balanced:

(1)x^2 + 16x + (1/4) = -17 + (1/4).

Simplify the equation: x^2 + 16x + 1/4 = -17/4 + 1/4.

Further simplify the right side by finding a common denominator: x^2 + 16x + 1/4 = -16/4.

Combine the constants on the right side: x^2 + 16x + 1/4 = -4.

Write the left side as a perfect square: (x + 8)^2 = -4.

Multiply both sides by 4 to isolate (x + 8)^2 on the left side: 4(x + 8)^2 = -4.

Take the square root of both sides, noting both the positive and negative square roots: x + 8 = ±√(-4).

Simplify the right side: x + 8 = ±(2i).

Continue simplifying: x + 8 = 2i or x + 8 = -2i.

Isolate x in both equations: x = 2i - 8 and x = -2i - 8.

Further simplify: x = -8 + 2i and x = -8 - 2i.

# Quadratic Formula 
To solve the quadratic equation -x^2 + 5x = 2 using the quadratic formula, you can follow these steps:

Write the equation in standard form (ax^2 + bx + c = 0):

-x^2 + 5x - 2 = 0

Identify the coefficients:

a = -1
b = 5
c = -2

Apply the quadratic formula:

The quadratic formula is given by:

x = (-b ± √(b² - 4ac)) / (2a)

Plug in the values of a, b, and c:

x = (-(5) ± √((5)² - 4(-1)(-2))) / (2(-1))

Simplify:

x = (-5 ± √(25 - 8)) / (-2)

x = (-5 ± √17) / (-2)

So, the solutions to the equation -x^2 + 5x = 2 are:

x = (-5 + √17) / 2

x = (-5 - √17) / 2

# Finding Discriminant and Type Of Solution 

To find the discriminant of the quadratic equation -x^2 - 6x - 9 = 0 and determine the number and type of solutions, you can use the discriminant formula and then consider any other possible cases. The discriminant formula is given as:

Discriminant (D) = b^2 - 4ac

Where a, b, and c are the coefficients of the quadratic equation ax^2 + bx + c = 0.

In the case of -x^2 - 6x - 9 = 0:

a = -1
b = -6
c = -9

Calculate the discriminant:
D = (-6)^2 - 4(-1)(-9) = 36 - 36 = 0

The discriminant is equal to 0.

Now, let's consider the possible types of solutions based on the discriminant value:

If the discriminant is greater than 0 (D > 0), there are two distinct real solutions.

If the discriminant is equal to 0 (D = 0), there is one real solution (a repeated root).

If the discriminant is less than 0 (D < 0), there are two complex (non-real) solutions.

In the case of -x^2 - 6x - 9 = 0, the discriminant is 0, so there is one real solution, but it's a repeated root.

The solutions are:

x = -3

# Nonlinear systems by substituion
> [!Important] 
> can use elmination and graphing too but those are easy
To solve the nonlinear system of equations using substitution:

Start with the two equations:
2x^2 - 2 = y
-2x + 2 = y

Express one of the equations in terms of the other variable. In this case, it's convenient to express the second equation in terms of y:
-2x + 2 = y

Now, substitute the expression for y from the second equation into the first equation:
2x^2 - 2 = (-2x + 2)

Solve for x:
2x^2 + 2x - 2 - 2 = 0
2x^2 + 2x - 4 = 0

Divide the equation by 2 to simplify it:
x^2 + x - 2 = 0

Factor the quadratic equation:
(x + 2)(x - 1) = 0

Set each factor equal to zero and solve for x:
x + 2 = 0 --> x = -2
x - 1 = 0 --> x = 1

So, the solutions for x are x = -2 and x = 1. To find the corresponding values of y, substitute these values of x back into either of the original equations. For example, using the first equation:

For x = -2:
2(-2)^2 - 2 = y
8 - 2 = y
y = 6

For x = 1:
2(1)^2 - 2 = y
2 - 2 = y
y = 0

The solutions to the system of equations are x = -2, y = 6, and x = 1, y = 0.
